rename with cat_ and remove superfluous assumptions
Signed-off-by: Ali Caglayan <alizter@gmail.com>

theories/WildCat/Products.v
@@ -7,42 +7,42 @@ Require Import WildCat.Core.
 
 Class HasBinaryProducts (A : Type) `{Is1Cat A} := {
   (** A binary product is an object of a category given by a pair of objects. *)
-  product : A -> A -> A;
+  cat_prod : A -> A -> A;
 
   (** It comes equipped with two projection maps out of the product. *)
-  cat_pr1 : forall {x y : A}, product x y $-> x;
-  cat_pr2 : forall {x y : A}, product x y $-> y;
+  cat_pr1 : forall {x y : A}, cat_prod x y $-> x;
+  cat_pr2 : forall {x y : A}, cat_prod x y $-> y;
   
   (** Together with a pairing "corecursor" into the product. *)
-  product_corec : forall {x y z : A},
-    (z $-> x) -> (z $-> y) -> (z $-> product x y);
+  cat_prod_corec : forall {x y z : A},
+    (z $-> x) -> (z $-> y) -> (z $-> cat_prod x y);
 
   (** All this data satisifies certain equiations, leading to the unqiueness of the product_corec map. *)
 
   (** Applying the first projection after a map pariing gives the first map. *) 
-  product_beta_pr1 {x y z : A} (f : z $-> x) (g : z $-> y)
-    : cat_pr1 $o product_corec f g $== f;
+  cat_prod_beta_pr1 {x y z : A} (f : z $-> x) (g : z $-> y)
+    : cat_pr1 $o cat_prod_corec f g $== f;
   
   (** Applying the second projection after a map pariing gives the second map. *)
-  product_beta_pr2 {x y z : A} (f : z $-> x) (g : z $-> y)
-    : cat_pr2 $o product_corec f g $== g;
+  cat_prod_beta_pr2 {x y z : A} (f : z $-> x) (g : z $-> y)
+    : cat_pr2 $o cat_prod_corec f g $== g;
 
   (** The pairing map is the unique map that makes the following diagram commute. *)
-  product_eta {x y z : A} (f : z $-> product x y)
-    : product_corec (cat_pr1 $o f) (cat_pr2 $o f) $== f;
+  cat_prod_eta {x y z : A} (f : z $-> cat_prod x y)
+    : cat_prod_corec (cat_pr1 $o f) (cat_pr2 $o f) $== f;
   
-  (** Finally given any two [product_corec], they are uniquely identified by their components. (This introduces a 2-categorical notion of product, which for n-categorical universal properties will need (n+1) levels of cells. We therefore restrict to 1-categories for now). Without this condition, we would not be able to show the 2-functorial action of the product functor or even 1-functoriality in the second argument. *) 
-  product_corec_eta {x y z : A} {f f' : z $-> x} {g g' : z $-> y}
-    : f $== f' -> g $== g' -> product_corec f g $== product_corec f' g';
+  (** Finally given any two [cat_prod_corec], they are uniquely identified by their components. (This introduces a 2-categorical notion of product, which for n-categorical universal properties will need (n+1) levels of cells. We therefore restrict to 1-categories for now). Without this condition, we would not be able to show the 2-functorial action of the product functor or even 1-functoriality in the second argument. *) 
+  cat_prod_corec_eta {x y z : A} {f f' : z $-> x} {g g' : z $-> y}
+    : f $== f' -> g $== g' -> cat_prod_corec f g $== cat_prod_corec f' g';
 }.
 
-Lemma product_pr_eta {A} `{HasBinaryProducts A}
-  {x y z : A} {f f' : z $-> product x y}
+Lemma cat_prod_pr_eta {A} `{HasBinaryProducts A}
+  {x y z : A} {f f' : z $-> cat_prod x y}
   : cat_pr1 $o f $== cat_pr1 $o f' -> cat_pr2 $o f $== cat_pr2 $o f' -> f $== f'.
 Proof.
   intros fst snd.
-  refine ((product_eta _)^$ $@ _ $@ product_eta _).
-  by apply product_corec_eta.
+  refine ((cat_prod_eta _)^$ $@ _ $@ cat_prod_eta _).
+  by apply cat_prod_corec_eta.
 Defined.
 
 (** In general it's not possible to define a recursor for a product. It is possible if a category has an internal hom, but that is a very strong condition.  *)
@@ -51,99 +51,105 @@ Defined.
 
 
 (** Binary products are functorial in each argument. *)
-Global Instance is0functor_product_l {A : Type} `{Is1Cat A} `{HasBinaryProducts A} y
-  : Is0Functor (fun x => product x y).
+Global Instance is0functor_cat_prod_l {A : Type}
+  `{HasBinaryProducts A} y
+  : Is0Functor (fun x => cat_prod x y).
 Proof.
   snrapply Build_Is0Functor.
   intros a b f.
-  apply product_corec.
+  apply cat_prod_corec.
   - exact (f $o cat_pr1).
   - exact cat_pr2.
 Defined.
 
-Global Instance is1functor_product_l {A : Type} `{Is1Cat A} `{HasBinaryProducts A} y
-  : Is1Functor (fun x => product x y).
+Global Instance is1functor_cat_prod_l {A : Type}
+  `{HasBinaryProducts A} y
+  : Is1Functor (fun x => cat_prod x y).
 Proof.
   snrapply Build_Is1Functor.
   - intros a b f g p.
     simpl.
-    apply product_corec_eta.
+    apply cat_prod_corec_eta.
     2: apply Id.
     exact (p $@R cat_pr1).
   - intros x.
     simpl.
-    apply product_pr_eta.
-    + refine (product_beta_pr1 _ _ $@ _).
+    apply cat_prod_pr_eta.
+    + refine (cat_prod_beta_pr1 _ _ $@ _).
       exact (cat_idl _ $@ (cat_idr _)^$).
-    + refine (product_beta_pr2 _ _ $@ _).
+    + refine (cat_prod_beta_pr2 _ _ $@ _).
       exact (cat_idr _)^$.
   - intros x z w f g.
     simpl.
-    apply product_pr_eta.
-    + refine (product_beta_pr1 _ _ $@ _).
+    apply cat_prod_pr_eta.
+    + refine (cat_prod_beta_pr1 _ _ $@ _).
       refine (_ $@ cat_assoc _ _ _).
-      refine (_ $@ ((product_beta_pr1 _ _)^$ $@R _)).
+      refine (_ $@ ((cat_prod_beta_pr1 _ _)^$ $@R _)).
       refine (cat_assoc _ _ _ $@ (_ $@L _) $@ (cat_assoc _ _ _)^$).
-      exact (product_beta_pr1 _ _)^$.
-    + refine (product_beta_pr2 _ _ $@ _).
+      exact (cat_prod_beta_pr1 _ _)^$.
+    + refine (cat_prod_beta_pr2 _ _ $@ _).
       refine (_ $@ cat_assoc _ _ _).
-      refine (_ $@ ((product_beta_pr2 _ _)^$ $@R _)).
-      exact (product_beta_pr2 _ _)^$.
+      refine (_ $@ ((cat_prod_beta_pr2 _ _)^$ $@R _)).
+      exact (cat_prod_beta_pr2 _ _)^$.
 Defined.
 
-Global Instance is0functor_product_r {A : Type} `{Is1Cat A} `{HasBinaryProducts A} x
-  : Is0Functor (product x).
+Global Instance is0functor_cat_prod_r {A : Type}
+  `{HasBinaryProducts A} x
+  : Is0Functor (cat_prod x).
 Proof.
   snrapply Build_Is0Functor.
   intros a b f.
-  apply product_corec.
+  apply cat_prod_corec.
   - exact cat_pr1.
   - exact (f $o cat_pr2).
 Defined.
 
-Global Instance is1functor_product_r {A : Type} `{Is1Cat A} `{HasBinaryProducts A} x
-  : Is1Functor (product x).
+Global Instance is1functor_cat_prod_r {A : Type}
+  `{HasBinaryProducts A} x
+  : Is1Functor (cat_prod x).
 Proof.
   snrapply Build_Is1Functor.
   - intros y z f g p.
-    apply product_corec_eta.
+    apply cat_prod_corec_eta.
     1: apply Id.
     exact (p $@R cat_pr2).
   - intros y. simpl.
-    refine (_ $@ product_eta _).
-    apply product_corec_eta.
+    refine (_ $@ cat_prod_eta _).
+    apply cat_prod_corec_eta.
     + symmetry.
       apply cat_idr.
     + exact (cat_idl _ $@ (cat_idr _)^$).
   - intros y z w f g.
     simpl.
-    apply product_pr_eta.
-    + refine (product_beta_pr1 _ _ $@ _).
+    apply cat_prod_pr_eta.
+    + refine (cat_prod_beta_pr1 _ _ $@ _).
       refine (_ $@ cat_assoc _ _ _).
-      refine (_ $@ ((product_beta_pr1 _ _)^$ $@R _)).
-      exact (product_beta_pr1 _ _)^$.    
-    + refine (product_beta_pr2 _ _ $@ _).
+      refine (_ $@ ((cat_prod_beta_pr1 _ _)^$ $@R _)).
+      exact (cat_prod_beta_pr1 _ _)^$.    
+    + refine (cat_prod_beta_pr2 _ _ $@ _).
       refine (_ $@ cat_assoc _ _ _).
-      refine (_ $@ ((product_beta_pr2 _ _)^$ $@R _)).
+      refine (_ $@ ((cat_prod_beta_pr2 _ _)^$ $@R _)).
       refine (_ $@ (cat_assoc _ _ _)^$).
       refine (cat_assoc _ _ _ $@ _).
-      exact (_ $@L product_beta_pr2 _ _)^$.
+      exact (_ $@L cat_prod_beta_pr2 _ _)^$.
 Defined.
 
-(** [product_corec] is also functorial in each morphsism. *)
+(** [cat_prod_corec] is also functorial in each morphsism. *)
 
-Global Instance is0functor_product_corec_l {A : Type} `{Is1Cat A} `{HasBinaryProducts A} {x y z : A} (g : z $-> y)
-  : Is0Functor (fun f => @product_corec _ _ _ _ _ _ x y z f g).
+Global Instance is0functor_cat_prod_corec_l {A : Type}
+  `{HasBinaryProducts A} {x y z : A} (g : z $-> y)
+  : Is0Functor (fun f => @cat_prod_corec _ _ _ _ _ _ x y z f g).
 Proof.
   snrapply Build_Is0Functor.
   intros f f' p.
-  by apply product_corec_eta.
+  by apply cat_prod_corec_eta.
 Defined.
 
-Global Instance is0functor_product_corec_r {A : Type} `{Is1Cat A} `{HasBinaryProducts A} {x y z : A} (f : z $-> x)
-  : Is0Functor (@product_corec _ _ _ _ _ _ x y z f).
+Global Instance is0functor_cat_prod_corec_r {A : Type}
+  `{HasBinaryProducts A} {x y z : A} (f : z $-> x)
+  : Is0Functor (@cat_prod_corec _ _ _ _ _ _ x y z f).
 Proof.
   snrapply Build_Is0Functor.
   intros g h p.
-  by apply product_corec_eta.
+  by apply cat_prod_corec_eta.
 Defined.
